case_study/RiscvPmpBoundedInts/Contracts.v
@@ -1535,7 +1535,7 @@ Module RiscvPmpValidContracts.
                  inversion H
              | |- _ => rewrite ?N_ltb_0 in *; try progress cbn
              end; cbn; auto.
-    all: apply pmp_check_perms_gives_access; first assumption.
+    all: apply pmp_check_perms_gives_access; assumption.
   Qed.
 
   (* TODO: this is just to make sure that all contracts defined so far are valid
